internalize atomic cut-elimination for ILL in semantics

coq.yalla/cut_elim.v
@@ -10,7 +10,8 @@
 Require Import List_more List_Type genperm_Type.
 
 Require Import orthogonality phase_sem rules_algebra.
-Require Import ill_cut_at.
+
+Require Import ill_def.
 
 Set Implicit Arguments.
 
@@ -45,104 +46,114 @@ Section Okada.
 
   Notation "↓" := (fun A Γ => ill P Γ A).
 
+(*
   Notation ILLval := (fun x => ↓(£x)).
+*)
+  Definition ILLval P := (fun X Γ => ( Γ = ivar X :: nil )
+                               + {a |  Γ = fst (projT2 (ipgax P) a) /\ ivar X = snd (projT2 (ipgax P) a) })%type.
 
   Fact ILLdc_closed: forall A, cl (↓A) ⊆ ↓A.
   Proof. apply dc_closed. Qed.
 
   Hint Resolve ILLdc_closed.
 
-  Fact ILLvdc_closed: forall x, cl (↓(£x)) ⊆ ↓(£x).
-  Proof. intros; apply ILLdc_closed. Qed.
-
   Hypothesis P_gax_noN_l : gax_noN_l P.
   Hypothesis P_gax_at_l : gax_at_l P.
   Hypothesis P_gax_at_r : gax_at_r P.
   Hypothesis P_gax_cut : gax_cut P.
 
-(* TODO replace lcompose by list_form_presem ??? *)
-  Let lcompose := fold_right (fun x y => composes PScompose x y) (sg PSunit).
-  Fact ILLgax : forall a, list_form_presem PSILL ILLval (fst (projT2 (ipgax P) a))
-                    ⊆ form_sem PSILL ILLval (snd (projT2 (ipgax P) a)).
+  Lemma atlist_from_gax : forall a, {l | fst (projT2 (ipgax P) a) = map ivar l }.
   Proof.
-    red in P_gax_at_l, P_gax_at_r.
-    intros a; specialize P_gax_at_l with a; specialize P_gax_at_r with a.
-    remember (snd (projT2 (ipgax P) a)) as b.
-    destruct b; inversion P_gax_at_r; simpl.
-    assert ({l : list IAtom | fst (projT2 (ipgax P) a) = map ivar l }) as [l Heq].
-    { revert P_gax_at_l ; remember (fst (projT2 (ipgax P) a)) as L; clear.
-      induction L; intros Hat.
-      - exists nil; reflexivity.
-      - inversion Hat; inversion H1; subst.
-        destruct (IHL H2) as [l Heq]; subst.
-        exists (x0 :: l); reflexivity. }
-    rewrite Heq.
-    replace (list_form_presem PSILL ILLval (map ivar l))
-       with (lcompose (map ILLval l))
-      by (clear; induction l; auto; simpl; rewrite IHl; auto).
-    apply subset_trans with (cl (lcompose (map ILLval l))).
-    { clear; induction l; try reflexivity.
-    - simpl; unfold ldual, rdual; simpl.
-      intros x H; unfold list_form_presem in H; simpl in H; subst.
-      unfold ctx_orth; intros [[de1 de2] A] H.
-      specialize H with nil; apply H; reflexivity.
-    - revert IHl; simpl.
-      remember (lcompose (map (fun x Γ => ill P Γ (£ x)) l)) as L1; clear HeqL1.
-      remember (lcompose (map (fun x Γ => ill P Γ (£ x)) l)) as L2; clear HeqL2.
-      remember (fun Γ : list iformula => ill P Γ (£ a)) as L0; clear HeqL0.
-      intros IH.
-      apply (@cl_increase _ _ (CL_ctx (ill P))). }
-    apply cl_closed; [ apply subset_preorder | apply dc_closed | ].
-    assert (ill P (nil ++ map ivar l) (ivar i)) as pi
-      by (rewrite Heqb; rewrite <- Heq; apply gax_ir).
-    apply subset_trans with (fun Γ => ill P (nil ++ Γ) (£ i)); [ | intros A H; auto ].
-    revert pi; remember nil as l0; clear Heql0.
-    revert l0; clear - P_gax_noN_l P_gax_cut; induction l; intros l0 pi.
-    + simpl; intros l Heq; subst; auto.
-    + intros Ga H.
-      inversion H; subst.
-      list_simpl in pi.
-      assert (pi' := @cut_at _ P_gax_noN_l P_gax_cut _ _ _ _ _ X pi).
-      rewrite app_assoc in pi'.
-      apply IHl in pi'.
-      apply pi' in X0.
-      rewrite <- app_assoc in X0; auto.
+  intros a.
+  red in P_gax_at_l.
+  specialize P_gax_at_l with a.
+  revert P_gax_at_l ; remember (fst (projT2 (ipgax P) a)) as L; clear.
+  induction L; intros Hat.
+  - exists nil; reflexivity.
+  - inversion Hat; inversion H1; subst.
+    destruct (IHL H2) as [l Heq]; subst.
+    exists (x0 :: l); reflexivity.
+  Qed.
+
+  Fact ILLgax : forall a, list_form_presem PSILL (ILLval P) (fst (projT2 (ipgax P) a))
+                    ⊆ cl(form_presem PSILL (ILLval P) (snd (projT2 (ipgax P) a))).
+  Proof.
+  intros.
+  etransitivity; [ | apply cl_increase ].
+  destruct (atlist_from_gax a) as [l Heq].
+  rewrite Heq.
+  red in P_gax_at_r; specialize P_gax_at_r with a.
+  remember (snd (projT2 (ipgax P) a)) as b.
+  destruct b; inversion P_gax_at_r; subst.
+  intros x Hx; right; rewrite Heqb.
+  enough (forall l0 a l1 l2, map ivar l1 ++ map ivar l0 = fst (projT2 (ipgax P) a) ->
+            list_form_presem PSILL (ILLval P) (map £ l0) l2 ->
+            { c | map ivar l1 ++ l2 = fst (projT2 (ipgax P) c)
+               /\ snd (projT2 (ipgax P) a) = snd (projT2 (ipgax P) c) }).
+  { specialize X with l a nil x; list_simpl in X.
+    symmetry in Heq; apply X in Heq; auto. }
+  clear - P_gax_at_l P_gax_cut; induction l0; intros a' l1 l2 Heq Hsem; inversion Hsem; subst.
+  - list_simpl in Heq.
+    exists a'; split; list_simpl; auto.
+  - simpl in X; destruct X; subst.
+    + apply IHl0 with (a:=a') (l1 := l1 ++ a :: nil) in X0; list_simpl; auto.
+      list_simpl in X0; destruct X0 as [c [Heq1 Heq2]].
+      exists c; auto.
+    + destruct s as [c [Heq1 Heq2]]; subst.
+      red in P_gax_cut.
+      specialize P_gax_cut with c a' (map ivar l1) (map ivar l0).
+      rewrite <- Heq2 in P_gax_cut.
+      symmetry in Heq; apply P_gax_cut in Heq.
+      destruct Heq as [d [Heq3 Heq4]].
+      destruct (atlist_from_gax c) as [l' Heq'].
+      rewrite_all Heq'.
+      apply IHl0 with (a:=d) (l1 := l1 ++ l') in X0; list_simpl; auto.
+      list_simpl in X0; destruct X0 as [e [Heq5 Heq6]].
+      exists e; split; auto.
+      etransitivity; eassumption.
   Qed.
 
   Instance PMILL : PhaseModel P := {
     PMPS := PSILL;
-    PMval := ILLval;
-    PMval_closed := ILLvdc_closed;
-    PMgax := ILLgax
-  }.
+    PMval := ILLval P;
+    PMgax := ILLgax }.
 
   Infix "∘" := (composes PScompose) (at level 50, no associativity).
   Infix "⊸" := (magicwand_l PScompose) (at level 51, right associativity).
   Infix "⟜" := (magicwand_r PScompose) (at level 53, left associativity).
   Notation v := PMval.
-  Notation Hv := PMval_closed.
-  Notation "⟦ A ⟧" := (form_sem PSILL ILLval A) (at level 49).
-
-  Let cl_sem_closed A : cl (⟦A⟧) ⊆ ⟦A⟧.
-  Proof. apply (@form_sem_closed _ PMILL); auto. Qed.
+  Notation "⟦ A ⟧" := (form_presem PSILL (ILLval P) A) (at level 49).
 
   Section Okada_Lemma.
 
-    Let cl_under_closed X Y : cl Y ⊆ Y -> X ⊆ Y -> cl X ⊆ Y.
+    Let ILLcl_closed X Y : cl Y ⊆ Y -> X ⊆ Y -> cl X ⊆ Y.
     Proof. apply cl_closed; apply subset_preorder. Qed.
 
-    Lemma Okada_formula A : ((sg (A::nil) ⊆ ⟦A⟧) * (⟦A⟧ ⊆ ↓A))%type.
+    Notation ILLcl_increase := (@cl_increase _ _ (CL_ctx (ill P))).
+
+
+    Lemma Okada_var_1 : forall X, sg (ivar X :: nil) ⊆ ⟦ivar X⟧.
+    Proof. intros X x Hx; subst; left; reflexivity. Qed.
+
+    Lemma Okada_var_2 : forall X, ⟦ivar X⟧ ⊆ ↓(ivar X).
+    Proof.
+    intros X x Hx; inversion Hx; subst.
+    - apply ax_ir.
+    - destruct X0 as [a [Heq1 Heq2]]; subst; rewrite Heq2.
+      apply gax_ir.
+    Qed.
+
+    Lemma Okada_formula A : ((sg (A :: nil) ⊆ ⟦A⟧) * (⟦A⟧ ⊆ ↓A))%type.
     Proof.
     induction A; simpl;
       try (destruct IHA as [IHA01 IHA02]);
       try (destruct IHA1 as [IHA11 IHA12]);
       try (destruct IHA2 as [IHA21 IHA22]);
      (split; [ |
-      try (try (apply cl_under_closed; auto);
+      try (try (apply ILLcl_closed; auto);
            intros x Hx; inversion Hx; subst; constructor; auto; fail)]).
-    - intros x Hx; subst.
-      apply ax_ir.
-    - reflexivity.
+    - apply Okada_var_1.
+    - apply Okada_var_2.
     - unfold ldual, rdual, ctx_orth.
       intros x Hx [[de1 de2] A] Hy; subst; simpl.
       constructor.
@@ -155,8 +166,8 @@ Section Okada.
     - unfold magicwand_r.
       intros x Hx y Hy; subst.
       inversion Hy; subst.
-      enough (sg (A2 o- A1 :: b) ⊆ ⟦A2⟧) as Hi by (apply Hi; reflexivity).
-      apply cl_under_closed in IHA21; auto.
+      enough (sg (A2 o- A1 :: b) ⊆ cl(⟦A2⟧)) as Hi by (apply Hi; reflexivity).
+      apply cl_monotone in IHA21; auto.
       etransitivity; [ | apply IHA21 ].
       intros x Hx; subst.
       unfold cl; simpl; unfold ldual, rdual, ctx_orth.
@@ -164,19 +175,36 @@ Section Okada.
       apply lpam_ilr; auto.
       specialize H with (A2 :: nil); apply H; auto.
     - intros x Hx; constructor.
+      apply ILLcl_closed in IHA22; [ | apply ILLdc_closed ].
       apply IHA22, Hx; constructor; auto.
     - unfold magicwand_r.
+      intros x Hx y Hy; subst.
+      inversion Hy; subst.
+      enough (sg (igen A :: b) ⊆ cl(⟦N⟧)) as Hi by (apply Hi; reflexivity).
+      assert (IHN := @Okada_var_1 atN).
+      apply cl_monotone in IHN; auto.
+      etransitivity; [ | apply IHN ].
+      intros x Hx; subst.
+      unfold cl; simpl; unfold ldual, rdual, ctx_orth.
+      intros [[si1 si2] C] H; simpl.
+      apply gen_pam_rule; auto.
+      specialize H with (N :: nil); apply H; auto.
+(* TODO simplify ???
+      unfold magicwand_r.
       intros x Hx y Hy; subst.
       inversion Hy; subst; simpl.
       apply gen_ilr.
       apply IHA02; auto.
+*)
     - intros x Hx; constructor.
-      apply Hx; constructor; auto.
+      assert (IHN := @Okada_var_2 atN).
+      apply ILLcl_closed in IHN; [ | apply ILLdc_closed ].
+      apply IHN, Hx; constructor; auto.
     - unfold magicwand_l.
       intros x Hx y Hy; subst.
       inversion Hy; subst.
-      enough (sg (a ++ A1 -o A2 :: nil) ⊆ ⟦A2⟧) as Hi by (apply Hi; reflexivity).
-      apply cl_under_closed in IHA21; auto.
+      enough (sg (a ++ A1 -o A2 :: nil) ⊆ cl(⟦A2⟧)) as Hi by (apply Hi; reflexivity).
+      apply cl_monotone in IHA21; auto.
       etransitivity; [ | apply IHA21 ].
       intros x Hx; subst.
       unfold cl; simpl; unfold ldual, rdual, ctx_orth.
@@ -184,32 +212,57 @@ Section Okada.
       apply lmap_ilr; auto.
       specialize H with (A2 :: nil); apply H; auto.
     - intros x Hx; constructor.
+      apply ILLcl_closed in IHA22; [ | apply ILLdc_closed ].
       apply IHA22, Hx.
       change (A1 :: x) with ((A1 :: nil) ++ x); constructor; auto.
     - unfold magicwand_l.
       intros x Hx y Hy; subst.
+      inversion Hy; subst.
+      enough (sg (a ++ ineg A :: nil) ⊆ cl(⟦N⟧)) as Hi by (apply Hi; reflexivity).
+      assert (IHN := @Okada_var_1 atN).
+      apply cl_monotone in IHN; auto.
+      etransitivity; [ | apply IHN ].
+      intros x Hx; subst.
+      unfold cl; simpl; unfold ldual, rdual, ctx_orth.
+      intros [[si1 si2] C] H; list_simpl.
+      apply neg_map_rule; auto.
+      specialize H with (N :: nil); apply H; auto.
+(* TODO simplify ???
+      unfold magicwand_l.
+      intros x Hx y Hy; subst.
       inversion Hy; subst; simpl.
       apply neg_ilr.
       apply IHA02; auto.
+*)
     - intros x Hx; constructor.
-      apply Hx.
+      assert (IHN := @Okada_var_2 atN).
+      apply ILLcl_closed in IHN; [ | apply ILLdc_closed ].
+      apply IHN, Hx.
       change (A :: x) with ((A :: nil) ++ x); constructor; auto.
     - apply top_greatest.
     - apply glb_in.
-      + apply cl_under_closed in IHA11; auto.
+      + apply cl_monotone in IHA11; auto.
         etransitivity; [ | apply IHA11 ].
         intros x Hx; subst.
         unfold cl; simpl; unfold ldual, rdual, ctx_orth.
         intros [[si1 si2] C] H; simpl.
         apply with_ilr1.
         specialize H with (A1 :: nil); apply H; auto.
-      + apply cl_under_closed in IHA21; auto.
+      + apply cl_monotone in IHA21; auto.
         etransitivity; [ | apply IHA21 ].
         intros x Hx; subst.
         unfold cl; simpl; unfold ldual, rdual, ctx_orth.
         intros [[si1 si2] C] H; simpl.
         apply with_ilr2.
         specialize H with (A2 :: nil); apply H; auto.
+    - unfold ldual, rdual, ctx_orth.
+      intros x Hx; inversion Hx; subst; constructor; auto.
+      + specialize X with (nil,nil,A1); list_simpl in X; apply X.
+        intros y Hy; list_simpl.
+        apply IHA12; auto.
+      + specialize X0 with (nil,nil,A2); list_simpl in X0; apply X0.
+        intros y Hy; list_simpl.
+        apply IHA22; auto.
     - unfold ldual, rdual, ctx_orth.
       intros x Hx [[de1 de2] A] Hy; subst; simpl.
       constructor.
@@ -223,23 +276,27 @@ Section Okada.
       specialize Hy with (!A :: nil); apply Hy; auto.
       split.
       + exists (A :: nil); reflexivity.
-      + enough (sg (!A :: nil) ⊆ ⟦A⟧) as Hoc by (apply Hoc; reflexivity).
-        apply cl_under_closed in IHA01; auto.
+      + enough (sg (!A :: nil) ⊆ cl(⟦A⟧)) as Hoc by (apply Hoc; reflexivity).
+        apply cl_monotone in IHA01; auto.
         etransitivity; [ | apply IHA01 ].
         intros x Hx; subst.
         unfold cl; simpl; unfold ldual, rdual, ctx_orth.
         intros [[si1 si2] C] H; simpl.
         apply de_ilr.
         specialize H with (A :: nil); apply H; auto.
-    - apply cl_under_closed; auto.
+    - apply ILLcl_closed; auto.
       intros x Hx; inversion Hx; subst.
       inversion H; subst.
       constructor; auto.
+      unfold ldual, rdual, ctx_orth in X.
+      specialize X with (nil,nil,A); list_simpl in X; apply X.
+      intros y Hy; list_simpl.
+      apply IHA02; auto.
     Qed.
 
   End Okada_Lemma.
 
-  Notation "⟬߭ Γ ⟭" := (list_form_presem PSILL ILLval Γ) (at level 49).
+  Notation "⟬߭ Γ ⟭" := (list_form_presem PSILL (ILLval P) Γ) (at level 49).
 
   (* We lift the result to contexts, ie list of formulas *)
 
@@ -273,16 +330,17 @@ Section cut_admissibility.
   (* Coercion: the phase model relying on cut-free provability over P is a phase model for P *)
   Instance PMILL_cfat : PhaseModel P := {
     PMPS := PSILL_cfat;
-    PMval := fun x ga => ill (cutupd_ipfrag P false) ga (£x);
-    PMval_closed :=  @ILLvdc_closed (cutupd_ipfrag P false);
-    PMgax := @ILLgax (cutupd_ipfrag P false) P_gax_noN_l P_gax_at_l P_gax_at_r P_gax_cut
-  }.
+    PMval := ILLval (cutupd_ipfrag P false);
+    PMgax := @ILLgax (cutupd_ipfrag P false) P_gax_at_l P_gax_at_r P_gax_cut }.
 
   Theorem ill_cut_elimination Γ A : Γ ⊢ A [P] -> Γ ⊢ A [cutupd_ipfrag P false].
   Proof.
     intros pi.
     apply (ill_soundness PMILL_cfat) in pi; auto.
-    apply Okada_formula, pi, Okada_ctx; auto.
+    assert (gax_noN_l (cutupd_ipfrag P false)) as HgaxN_cf by assumption.
+    assert (HO := snd (Okada_formula HgaxN_cf A)).
+    apply (@cl_closed _ _ _ CL_cfat) in HO; [ | apply dc_closed ].
+    apply HO, pi, Okada_ctx; auto.
   Qed.
 
 End cut_admissibility.
